@prefix aamva_d20:      <https://docs.oasis-open.org/niemopen/ns/model/codes/aamva_d20/6.0/> .
@prefix exch:           <http://example.com/CrashDriver/1.3/> .
@prefix gml:            <http://www.opengis.net/gml/3.2> .
@prefix hs:             <https://docs.oasis-open.org/niemopen/ns/model/domains/humanServices/6.0/> .
@prefix j:              <https://docs.oasis-open.org/niemopen/ns/model/domains/justice/6.0/> .
@prefix nc:             <https://docs.oasis-open.org/niemopen/ns/model/niem-core/6.0/> .
@prefix niem-gml:       <https://docs.oasis-open.org/niemopen/ns/model/adapters/niem-gml/6.0/> .
@prefix priv:           <http://example.com/PrivacyMetadata/2.0/> .
@prefix xs:             <http://www.w3.org/2001/XMLSchema> .

@prefix owl:            <http://www.w3.org/2002/07/owl#> .
@prefix rdfs:           <http://www.w3.org/2000/01/rdf-schema#> .
@prefix rdf:            <http://www.w3.org/1999/02/22-rdf-syntax-ns#> .
@prefix xsd:            <http://www.w3.org/2001/XMLSchema> .

priv:privacyRelationCode
    a owl:DataProperty ;
    rdfs:range priv:PrivacyCodeType .

j:CrashDriver
    a owl:ObjectProperty ;
    rdfs:range j:CrashDriverType ;
    rdfs:comment "A motor vehicle driver involved into a traffic accident." .

exch:ReferenceObjects
    a owl:ObjectProperty ;
    rdfs:range exch:ReferenceObjectType ;
    rdfs:comment "Objects that do not apply to their parent (and appear only by reference)." .

nc:ActivityDate
    a owl:ObjectProperty ;
    rdfs:range nc:DateType ;
    rdfs:comment "A date of an activity." .

j:PersonChargeAssociation
    a owl:ObjectProperty ;
    rdfs:range j:PersonChargeAssociationType ;
    rdfs:comment "An association between a person and a charge issued to that person." .

nc:InjuryDescriptionText
    a owl:DataProperty ;
    rdfs:range nc:TextType ;
    rdfs:comment "A description of an injury." .

nc:PersonUnionAssociation
    a owl:ObjectProperty ;
    rdfs:range nc:PersonUnionAssociationType ;
    rdfs:comment "An association between two persons who are in a state of union with each other." .

nc:PersonNameSalutationText
    a owl:DataProperty ;
    rdfs:range nc:TextType ;
    rdfs:comment "A formal sign or expression of greeting that is appropriate for this person." .

nc:PersonSurName
    a owl:DataProperty ;
    rdfs:range nc:PersonNameTextType ;
    rdfs:comment "A last name or family name of a person." .

j:CrashPerson
    a owl:ObjectProperty ;
    rdfs:range j:CrashPersonType ;
    rdfs:comment "A person involved in a traffic accident." .

exch:PersonFictionalGenreCodeLiteral
    a owl:DataProperty ;
    rdfs:range exch:PersonFictionalGenreCodeSimpleType ;
    rdfs:comment "A data type for the genre of a fictional character." .

priv:PrivacyCode
    a owl:DataProperty ;
    rdfs:range priv:PrivacyCodeType .

nc:PersonMiddleName
    a owl:DataProperty ;
    rdfs:range nc:PersonNameTextType ;
    rdfs:comment "A middle name of a person." .

exch:PersonFictionalGenreCode
    a owl:ObjectProperty ;
    rdfs:range exch:PersonFictionalGenreCodeType ;
    rdfs:comment "A genre of a fictional character." .

j:InjurySeverityCode
    a owl:DataProperty ;
    rdfs:range aamva_d20:AccidentSeverityCodeType ;
    rdfs:comment "A severity of an injury received by a person, such as in a traffic accident or crash." .

priv:PrivacyMetadata
    a owl:ObjectProperty ;
    rdfs:range priv:PrivacyMetadataType .

exch:PersonFictionalCharacterIndicator
    a owl:DataProperty ;
    rdfs:range xsd:boolean ;
    rdfs:comment "True if this person is a fictional character in a literary work; false otherwise." .

nc:GeographicCoordinateLatitude
    a owl:ObjectProperty ;
    rdfs:range nc:LatitudeCoordinateType ;
    rdfs:comment "A measurement of the angular distance between a point on the Earth and the Equator." .

nc:PersonBirthDate
    a owl:ObjectProperty ;
    rdfs:range nc:DateType ;
    rdfs:comment "A date a person was born." .

nc:SourceIDText
    a owl:DataProperty ;
    rdfs:range nc:TextType ;
    rdfs:comment "A number or string set by a data provider so that information that is sent can be retraced back to its source." .

nc:GeographicCoordinateLongitude
    a owl:ObjectProperty ;
    rdfs:range nc:LongitudeCoordinateType ;
    rdfs:comment "A measurement of the angular distance between a point on the Earth and the Prime Meridian." .

hs:PersonOtherKinAssociationCategoryText
    a owl:DataProperty ;
    rdfs:range nc:TextType ;
    rdfs:comment "A kind of kinship or other close personal relationship that exists from the source person to the target person." .

nc:personNameCommentText
    a owl:DataProperty ;
    rdfs:range xsd:string ;
    rdfs:comment "A comment about a kind of name for a person." .

j:Charge
    a owl:ObjectProperty ;
    rdfs:range j:ChargeType ;
    rdfs:comment "A formal allegation that a specific person has committed a specific offense." .

hs:PersonOtherKinAssociation
    a owl:ObjectProperty ;
    rdfs:range hs:PersonOtherKinAssociationType ;
    rdfs:comment "A directed association that describes the kinship or other close personal relationship between the source object and the target object. The relationship between a parent and a child should be captured using the ParentChildAssociation" .

nc:MeasureValueText
    a owl:DataProperty ;
    rdfs:range nc:TextType ;
    rdfs:comment "A textual description of a measurement value." .

j:PersonAdultIndicator
    a owl:DataProperty ;
    rdfs:range xsd:boolean ;
    rdfs:comment "True if person is considered an adult, based on age/emancipation/etc.; false otherwise." .

j:CrashVehicle
    a owl:ObjectProperty ;
    rdfs:range j:CrashVehicleType ;
    rdfs:comment "A motor vehicle involved in a traffic accident." .

j:CrashPersonInjury
    a owl:ObjectProperty ;
    rdfs:range nc:InjuryType ;
    rdfs:comment "An injury received by a person involved in a traffic accident." .

nc:PersonGivenName
    a owl:DataProperty ;
    rdfs:range nc:PersonNameTextType ;
    rdfs:comment "A first name of a person." .

nc:Date
    a owl:DataProperty ;
    rdfs:range xsd:date ;
    rdfs:comment "A full date." .

j:IntelligenceInformationIndicator
    a owl:DataProperty ;
    rdfs:range xsd:boolean ;
    rdfs:comment "True if the information specified is intelligence information; false otherwise." .

j:JuvenileAsAdultIndicator
    a owl:DataProperty ;
    rdfs:range xsd:boolean ;
    rdfs:comment "True if a juvenile is to be processed as an adult; false otherwise." .

niem-gml:LocationGeospatialPointAdapter
    a owl:ObjectProperty ;
    rdfs:subPropertyOf nc:LocationGeospatialCoordinateAbstract ;
    rdfs:range niem-gml:PointAdapterType ;
    rdfs:comment "A 2D or 3D geometric point.  A gml:Point is defined by a single coordinate tuple. The direct position of a point is specified by the gml:pos element which is of type gml:DirectPositionType." .

j:DriverLicense
    a owl:ObjectProperty ;
    rdfs:range j:DriverLicenseType ;
    rdfs:comment "A license issued to a person granting driving privileges." .

hs:TargetPerson
    a owl:ObjectProperty ;
    rdfs:range nc:PersonType ;
    rdfs:comment "A person that represents the end point of a directed association" .

nc:LongitudeDegreeValue
    a owl:DataProperty ;
    rdfs:range nc:LongitudeDegreeType ;
    rdfs:comment "A value that specifies the degree of a longitude. The value comes from a restricted range between -180 (inclusive) and +180 (inclusive)." .

nc:Metadata
    a owl:ObjectProperty ;
    rdfs:range nc:MetadataType ;
    rdfs:comment "Information that further qualifies primary data; data about data." .

j:ChargeDescriptionText
    a owl:DataProperty ;
    rdfs:range nc:TextType ;
    rdfs:comment "A plain language description of a charge." .

j:CriminalInformationIndicator
    a owl:DataProperty ;
    rdfs:range xsd:boolean ;
    rdfs:comment "True if the information specified is classified as criminal information; false if it is not classified as criminal information." .

nc:IdentificationID
    a owl:DataProperty ;
    rdfs:range xsd:string ;
    rdfs:comment "An identifier." .

nc:PersonUnionCategoryText
    a owl:DataProperty ;
    rdfs:range nc:TextType ;
    rdfs:comment "A kind of union between two people." .

j:DriverLicenseCardIdentification
    a owl:ObjectProperty ;
    rdfs:range nc:IdentificationType ;
    rdfs:comment "An identification that is affixed to the raw materials (card stock, laminate, etc.) used in producing driver licenses and ID cards. The numbers are issued by the material's manufacturer and provide a unique reference to a card within a jurisdiction." .

nc:ActivityLocation
    a owl:ObjectProperty ;
    rdfs:range nc:LocationType ;
    rdfs:comment "A location of an activity." .

nc:MeasureDecimalValue
    a owl:DataProperty ;
    rdfs:range xsd:decimal ;
    rdfs:comment "A decimal measurement value." .

hs:HouseholdMemberIndicator
    a owl:DataProperty ;
    rdfs:range xsd:boolean ;
    rdfs:comment "True if the associated person is a household member; false otherwise." .

j:Crash
    a owl:ObjectProperty ;
    rdfs:range j:CrashType ;
    rdfs:comment "A traffic accident." .

j:ChargeFelonyIndicator
    a owl:DataProperty ;
    rdfs:range xsd:boolean ;
    rdfs:comment "True if a charge refers to a felony offense; false otherwise." .

nc:ItemLengthMeasure
    a owl:ObjectProperty ;
    rdfs:range nc:LengthMeasureType ;
    rdfs:comment "A measurement of the length of an item." .

nc:Person
    a owl:ObjectProperty ;
    rdfs:range nc:PersonType ;
    rdfs:comment "A human being." .

nc:LatitudeDegreeValue
    a owl:DataProperty ;
    rdfs:range nc:LatitudeDegreeType ;
    rdfs:comment "A value that specifies the degree of a latitude. The value comes from a restricted range between -90 (inclusive) and +90 (inclusive)." .

hs:PersonOtherKinAssociationCategoryCode
    a owl:DataProperty ;
    rdfs:range hs:PersonOtherKinAssociationCodeType ;
    rdfs:comment "A code list that describes the nature of the kinship or other close personal relationship from a source person to a target person." .

exch:CrashDriverInfo
    a owl:ObjectProperty ;
    rdfs:range exch:CrashDriverInfoType ;
    rdfs:comment "A collection of legal charges associated with the driver of a vehicle in a crash." .

nc:PersonName
    a owl:ObjectProperty ;
    rdfs:range nc:PersonNameType ;
    rdfs:comment "A combination of names and/or titles by which a person is known." .

nc:ReportedDate
    a owl:ObjectProperty ;
    rdfs:range nc:DateType ;
    rdfs:comment "A date information was observed, measured, identified, or became known." .

nc:Location2DGeospatialCoordinate
    a owl:ObjectProperty ;
    rdfs:subPropertyOf nc:LocationGeospatialCoordinateAbstract ;
    rdfs:range nc:Location2DGeospatialCoordinateType ;
    rdfs:comment "A location identified by a latitude and longitude." .

hs:SourcePerson
    a owl:ObjectProperty ;
    rdfs:range nc:PersonType ;
    rdfs:comment "A person that is the start point of a directed association" .

nc:YearDate
    a owl:DataProperty ;
    rdfs:range xsd:gYear ;
    rdfs:comment "A year." .

j:CrashDriverType
    a owl:Class ;
    rdfs:subClass nc:PersonType ;
    rdfs:comment "A data type for a motor vehicle driver involved in a traffic accident." .

nc:PersonNameType
    a owl:Class ;
    rdfs:comment "A data type for a combination of names and/or titles by which a person is known." ;
    owl:subclassOf [
        a owl:Restriction ;
        owl:cardinality "1"^^xsd:nonNegativeInteger ;
        owl:onProperty nc:PersonGivenName
    ] ;
    owl:subclassOf [
        a owl:Restriction ;
        owl:cardinality "1"^^xsd:nonNegativeInteger ;
        owl:onProperty nc:PersonSurName
    ] .

hs:PersonOtherKinAssociationType
    a owl:Class ;
    rdfs:subClass nc:AssociationType ;
    rdfs:comment "A data type for a relationship that is a kinship or other close personal association between the source object and the target object. The relationship between a parent and a child should be captured using the ParentChildAssociation" ;
    owl:subclassOf [
        a owl:Restriction ;
        owl:cardinality "1"^^xsd:nonNegativeInteger ;
        owl:onProperty hs:SourcePerson
    ] ;
    owl:subclassOf [
        a owl:Restriction ;
        owl:cardinality "1"^^xsd:nonNegativeInteger ;
        owl:onProperty hs:TargetPerson
    ] ;
    owl:subclassOf [
        a owl:Restriction ;
        owl:minCardinality "1"^^xsd:nonNegativeInteger ;
        owl:onProperty hs:PersonOtherKinAssociationCategoryAbstract
    ] .

j:DrivingIncidentType
    a owl:Class ;
    rdfs:subClass nc:IncidentType ;
    rdfs:comment "A data type for details of an incident involving a vehicle." .

priv:PrivacyMetadataType
    a owl:Class ;
    owl:subclassOf [
        a owl:Restriction ;
        owl:minCardinality "1"^^xsd:nonNegativeInteger ;
        owl:onProperty priv:PrivacyCode
    ] .

j:CrashVehicleType
    a owl:Class ;
    rdfs:comment "A data type for a motor vehicle involved in a traffic accident." ;
    owl:subclassOf [
        a owl:Restriction ;
        owl:cardinality "1"^^xsd:nonNegativeInteger ;
        owl:onProperty j:CrashDriver
    ] .

j:DriverLicenseBaseType
    a owl:Class ;
    rdfs:comment "A data type for an authorization issued to a driver granting driving privileges." .

exch:PersonFictionalGenreCodeType
    a owl:Class ;
    rdfs:comment "A data type for the genre of a fictional character." ;
    owl:subclassOf [
        a owl:Restriction ;
        owl:cardinality "1"^^xsd:nonNegativeInteger ;
        owl:onProperty exch:PersonFictionalGenreCodeLiteral
    ] .

nc:DateType
    a owl:Class ;
    rdfs:comment "A data type for a calendar date." ;
    owl:subclassOf [
        a owl:Restriction ;
        owl:cardinality "1"^^xsd:nonNegativeInteger ;
        owl:onProperty nc:DateRepresentation
    ] .

nc:MetadataType
    a owl:Class ;
    rdfs:comment "A data type for information that further qualifies primary data; data about data." .

nc:AssociationType
    a owl:Class ;
    rdfs:comment "A data type for an association, connection, relationship, or involvement somehow linking people, things, and/or activities together." .

j:DriverLicenseType
    a owl:Class ;
    rdfs:subClass j:DriverLicenseBaseType ;
    rdfs:comment "A data type for a license issued to a person granting driving privileges." ;
    owl:subclassOf [
        a owl:Restriction ;
        owl:cardinality "1"^^xsd:nonNegativeInteger ;
        owl:onProperty j:DriverLicenseCardIdentification
    ] .

nc:ActivityType
    a owl:Class ;
    rdfs:comment "A data type for a single or set of related actions, events, or process steps." .

niem-gml:PointAdapterType
    a owl:Class ;
    rdfs:comment "A data type for a 2D or 3D geometric point.  A gml:Point is defined by a single coordinate tuple. The direct position of a point is specified by the gml:pos element which is of type gml:DirectPositionType." ;
    owl:subclassOf [
        a owl:Restriction ;
        owl:cardinality "1"^^xsd:nonNegativeInteger ;
        owl:onProperty gml:Point
    ] .

exch:ReferenceObjectType
    a owl:Class ;
    rdfs:comment "A data type for objects that do not apply to their parent (and appear only by reference)." .

j:CrashType
    a owl:Class ;
    rdfs:subClass j:DrivingIncidentType ;
    rdfs:comment "A data type for a traffic accident." ;
    owl:subclassOf [
        a owl:Restriction ;
        owl:minCardinality "1"^^xsd:nonNegativeInteger ;
        owl:onProperty j:CrashVehicle
    ] ;
    owl:subclassOf [
        a owl:Restriction ;
        owl:minCardinality "1"^^xsd:nonNegativeInteger ;
        owl:onProperty j:CrashPerson
    ] .

nc:LatitudeCoordinateType
    a owl:Class ;
    rdfs:comment "A data type for a measurement of the angular distance between a point on the Earth and the Equator." ;
    owl:subclassOf [
        a owl:Restriction ;
        owl:cardinality "1"^^xsd:nonNegativeInteger ;
        owl:onProperty nc:LatitudeDegreeValue
    ] .

nc:LengthMeasureType
    a owl:Class ;
    rdfs:subClass nc:MeasureType ;
    rdfs:comment "A data type for a measure of a distance or extent." ;
    owl:subclassOf [
        a owl:Restriction ;
        owl:cardinality "1"^^xsd:nonNegativeInteger ;
        owl:onProperty nc:LengthUnitAbstract
    ] .

nc:MeasureType
    a owl:Class ;
    rdfs:comment "A data type for a measurement." ;
    owl:subclassOf [
        a owl:Restriction ;
        owl:cardinality "1"^^xsd:nonNegativeInteger ;
        owl:onProperty nc:MeasureValueAbstract
    ] .

j:ChargeType
    a owl:Class ;
    rdfs:comment "A data type for a formal allegation that a specific person has committed a specific offense." ;
    owl:subclassOf [
        a owl:Restriction ;
        owl:minCardinality "1"^^xsd:nonNegativeInteger ;
        owl:onProperty j:ChargeDescriptionText
    ] .

nc:PersonType
    a owl:Class ;
    rdfs:comment "A data type for a human being." .

nc:LongitudeCoordinateType
    a owl:Class ;
    rdfs:comment "A data type for a measurement of the angular distance between a point on the Earth and the Prime Meridian." ;
    owl:subclassOf [
        a owl:Restriction ;
        owl:cardinality "1"^^xsd:nonNegativeInteger ;
        owl:onProperty nc:LongitudeDegreeValue
    ] .

j:CrashPersonType
    a owl:Class ;
    rdfs:subClass nc:PersonType ;
    rdfs:comment "A data type for any person involved in a traffic accident." .

j:PersonChargeAssociationType
    a owl:Class ;
    rdfs:subClass nc:AssociationType ;
    rdfs:comment "A data type for an association between a person and a charge." ;
    owl:subclassOf [
        a owl:Restriction ;
        owl:cardinality "1"^^xsd:nonNegativeInteger ;
        owl:onProperty nc:Person
    ] ;
    owl:subclassOf [
        a owl:Restriction ;
        owl:cardinality "1"^^xsd:nonNegativeInteger ;
        owl:onProperty j:Charge
    ] .

nc:IdentificationType
    a owl:Class ;
    rdfs:comment "A data type for a representation of an identity." ;
    owl:subclassOf [
        a owl:Restriction ;
        owl:cardinality "1"^^xsd:nonNegativeInteger ;
        owl:onProperty nc:IdentificationID
    ] .

nc:InjuryType
    a owl:Class ;
    rdfs:comment "A data type for a form of harm or damage sustained by a person." ;
    owl:subclassOf [
        a owl:Restriction ;
        owl:cardinality "1"^^xsd:nonNegativeInteger ;
        owl:onProperty nc:InjuryDescriptionText
    ] ;
    owl:subclassOf [
        a owl:Restriction ;
        owl:cardinality "1"^^xsd:nonNegativeInteger ;
        owl:onProperty nc:InjurySeverityAbstract
    ] .

nc:Location2DGeospatialCoordinateType
    a owl:Class ;
    rdfs:comment "A data type for a location identified by latitude and longitude." ;
    owl:subclassOf [
        a owl:Restriction ;
        owl:cardinality "1"^^xsd:nonNegativeInteger ;
        owl:onProperty nc:GeographicCoordinateLatitude
    ] ;
    owl:subclassOf [
        a owl:Restriction ;
        owl:cardinality "1"^^xsd:nonNegativeInteger ;
        owl:onProperty nc:GeographicCoordinateLongitude
    ] .

exch:CrashDriverInfoType
    a owl:Class ;
    rdfs:comment "A data type for a collection of legal charges associated with the driver of a vehicle in a crash." ;
    owl:subclassOf [
        a owl:Restriction ;
        owl:cardinality "1"^^xsd:nonNegativeInteger ;
        owl:onProperty j:Crash
    ] .

nc:IncidentType
    a owl:Class ;
    rdfs:subClass nc:ActivityType ;
    rdfs:comment "A data type for an occurrence or an event that may require a response." .

nc:PersonAssociationType
    a owl:Class ;
    rdfs:subClass nc:AssociationType ;
    rdfs:comment "A data type for an association between people." .

nc:PersonUnionAssociationType
    a owl:Class ;
    rdfs:subClass nc:PersonAssociationType ;
    rdfs:comment "A data type for an association between two persons who are in a state of union with each other." .

nc:LocationType
    a owl:Class ;
    rdfs:comment "A data type for geospatial location." ;
    owl:subclassOf [
        a owl:Restriction ;
        owl:cardinality "1"^^xsd:nonNegativeInteger ;
        owl:onProperty nc:LocationGeospatialCoordinateAbstract
    ] .
