@prefix aamva_d20:      <https://docs.oasis-open.org/niemopen/ns/model/codes/aamva_d20/6.0/#> .
@prefix exch:           <http://example.com/CrashDriver/1.2/#> .
@prefix hs:             <https://docs.oasis-open.org/niemopen/ns/model/domains/humanServices/6.0/#> .
@prefix j:              <https://docs.oasis-open.org/niemopen/ns/model/domains/justice/6.0/#> .
@prefix nc:             <https://docs.oasis-open.org/niemopen/ns/model/niem-core/6.0/#> .
@prefix priv:           <http://example.com/PrivacyMetadata/2.0/#> .
@prefix xs:             <http://www.w3.org/2001/XMLSchema#> .

@prefix owl:            <http://www.w3.org/2002/07/owl##> .
@prefix rdfs:           <http://www.w3.org/2000/01/rdf-schema##> .
@prefix rdf:            <http://www.w3.org/1999/02/22-rdf-syntax-ns##> .
@prefix xsd:            <http://www.w3.org/2001/XMLSchema#> .

j:CrashDriver
    a owl:ObjectProperty ;
    rdfs:range j:CrashDriverType ;
    rdfs:comment "A motor vehicle driver involved into a traffic accident." .

nc:DateRepresentation
    a owl:DataProperty ;
    rdfs:comment "A data concept for a representation of a date." .

nc:ActivityDate
    a owl:ObjectProperty ;
    rdfs:range nc:DateType ;
    rdfs:comment "A date of an activity." .

j:PersonChargeAssociation
    a owl:ObjectProperty ;
    rdfs:range j:PersonChargeAssociationType ;
    rdfs:comment "An association between a person and a charge issued to that person." .

nc:InjuryDescriptionText
    a owl:DataProperty ;
    rdfs:range nc:TextType ;
    rdfs:comment "A description of an injury." .

nc:PersonUnionAssociation
    a owl:ObjectProperty ;
    rdfs:range nc:PersonUnionAssociationType ;
    rdfs:comment "An association between two persons who are in a state of union with each other." .

nc:PersonSurName
    a owl:DataProperty ;
    rdfs:range nc:PersonNameTextType ;
    rdfs:comment "A last name or family name of a person." .

j:CrashPerson
    a owl:ObjectProperty ;
    rdfs:range j:CrashPersonType ;
    rdfs:comment "A person involved in a traffic accident." .

priv:PrivacyCode
    a owl:DataProperty ;
    rdfs:range priv:PrivacyCodeType .

nc:PersonMiddleName
    a owl:DataProperty ;
    rdfs:range nc:PersonNameTextType ;
    rdfs:comment "A middle name of a person." .

j:InjurySeverityCode
    a owl:DataProperty ;
    rdfs:range aamva_d20:AccidentSeverityCodeType ;
    rdfs:comment "A severity of an injury received by a person, such as in a traffic accident or crash." .

priv:PrivacyMetadata
    a owl:ObjectProperty ;
    rdfs:range priv:PrivacyMetadataType .

nc:GeographicCoordinateLatitude
    a owl:ObjectProperty ;
    rdfs:range nc:LatitudeCoordinateType ;
    rdfs:comment "A measurement of the angular distance between a point on the Earth and the Equator." .

nc:PersonBirthDate
    a owl:ObjectProperty ;
    rdfs:range nc:DateType ;
    rdfs:comment "A date a person was born." .

nc:GeographicCoordinateLongitude
    a owl:ObjectProperty ;
    rdfs:range nc:LongitudeCoordinateType ;
    rdfs:comment "A measurement of the angular distance between a point on the Earth and the Prime Meridian." .

exch:CrashDriverInfo
    a owl:ObjectProperty ;
    rdfs:range exch:CrashDriverInfoType ;
    rdfs:comment "A collection of legal charges associated with the driver of a vehicle in a crash." .

exch:PersonFictionalCharacterIndicator
    a owl:DataProperty ;
    rdfs:range xsd:boolean ;
    rdfs:comment "True if this person is a fictional character in a literary work; false otherwise." .

hs:Child
    a owl:ObjectProperty ;
    rdfs:range hs:ChildType ;
    rdfs:comment "A person who was an unmarried minor at the time of his or her involvement in a judicial proceeding or non-judicial program." .

nc:personNameCommentText
    a owl:DataProperty ;
    rdfs:range xsd:string ;
    rdfs:comment "A comment about a kind of name for a person." .

hs:ParentChildAssociation
    a owl:ObjectProperty ;
    rdfs:range hs:ParentChildAssociationType ;
    rdfs:comment "An association between a child and a person who is in a parent role toward that child." .

j:Charge
    a owl:ObjectProperty ;
    rdfs:range j:ChargeType ;
    rdfs:comment "A formal allegation that a specific person has committed a specific offense." .

hs:PersonOtherKinAssociation
    a owl:ObjectProperty ;
    rdfs:range hs:PersonOtherKinAssociationType ;
    rdfs:comment "A directed association that describes the kinship or other close personal relationship between the source object and the target object. The relationship between a parent and a child should be captured using the ParentChildAssociation" .

nc:MeasureValueText
    a owl:DataProperty ;
    rdfs:range nc:TextType ;
    rdfs:comment "A textual description of a measurement value." .

nc:InjurySeverityAbstract
    a owl:DataProperty ;
    rdfs:comment "A data concept for a severity of an injury received by a person involved into a Traffic Accident." .

j:PersonAdultIndicator
    a owl:DataProperty ;
    rdfs:range xsd:boolean ;
    rdfs:comment "True if person is considered an adult, based on age/emancipation/etc.; false otherwise." .

j:CrashVehicle
    a owl:ObjectProperty ;
    rdfs:range j:CrashVehicleType ;
    rdfs:comment "A motor vehicle involved in a traffic accident." .

j:CrashPersonInjury
    a owl:ObjectProperty ;
    rdfs:range nc:InjuryType ;
    rdfs:comment "An injury received by a person involved in a traffic accident." .

nc:PersonGivenName
    a owl:DataProperty ;
    rdfs:range nc:PersonNameTextType ;
    rdfs:comment "A first name of a person." .

nc:Date
    a owl:DataProperty ;
    rdfs:range xsd:date ;
    rdfs:comment "A full date." .

j:IntelligenceInformationIndicator
    a owl:DataProperty ;
    rdfs:range xsd:boolean ;
    rdfs:comment "True if the information specified is intelligence information; false otherwise." .

j:JuvenileAsAdultIndicator
    a owl:DataProperty ;
    rdfs:range xsd:boolean ;
    rdfs:comment "True if a juvenile is to be processed as an adult; false otherwise." .

priv:privacyMetadataRef
    a owl:DataProperty ;
    rdfs:range xsd:IDREFS .

j:DriverLicense
    a owl:ObjectProperty ;
    rdfs:range j:DriverLicenseType ;
    rdfs:comment "A license issued to a person granting driving privileges." .

hs:PersonOtherKinAssociationCategoryAbstract
    a owl:DataProperty ;
    rdfs:comment "A data concept for describing the kinship or other close personal relationship that exists from the source person to the target person." .

nc:LengthUnitAbstract
    a null ;
    rdfs:comment "A data concept for a unit of measure for length." .

nc:LongitudeDegreeValue
    a owl:DataProperty ;
    rdfs:range nc:LongitudeDegreeType ;
    rdfs:comment "A value that specifies the degree of a longitude. The value comes from a restricted range between -180 (inclusive) and +180 (inclusive)." .

nc:Metadata
    a owl:ObjectProperty ;
    rdfs:range nc:MetadataType ;
    rdfs:comment "Information that further qualifies primary data; data about data." .

j:ChargeDescriptionText
    a owl:DataProperty ;
    rdfs:range nc:TextType ;
    rdfs:comment "A plain language description of a charge." .

j:CriminalInformationIndicator
    a owl:DataProperty ;
    rdfs:range xsd:boolean ;
    rdfs:comment "True if the information specified is classified as criminal information; false if it is not classified as criminal information." .

nc:IdentificationID
    a owl:DataProperty ;
    rdfs:range xsd:string ;
    rdfs:comment "An identifier." .

j:DriverLicenseCardIdentification
    a owl:ObjectProperty ;
    rdfs:range nc:IdentificationType ;
    rdfs:comment "An identification that is affixed to the raw materials (card stock, laminate, etc.) used in producing driver licenses and ID cards. The numbers are issued by the material's manufacturer and provide a unique reference to a card within a jurisdiction." .

nc:ActivityLocation
    a owl:ObjectProperty ;
    rdfs:range nc:LocationType ;
    rdfs:comment "A location of an activity." .

hs:Parent
    a owl:ObjectProperty ;
    rdfs:range nc:PersonType ;
    rdfs:comment "A father or mother of a person." .

nc:LocationGeospatialCoordinateAbstract
    a owl:ObjectProperty ;
    rdfs:comment "A data concept for a geospatial location." .

nc:MeasureValueAbstract
    a owl:DataProperty ;
    rdfs:comment "A data concept for a measurement value." .

nc:MeasureDecimalValue
    a owl:DataProperty ;
    rdfs:range xsd:decimal ;
    rdfs:comment "A decimal measurement value." .

nc:metadataRef
    a owl:DataProperty ;
    rdfs:range xsd:IDREFS ;
    rdfs:comment "A list of metadata objects that apply to a node or object represented by an XML element." .

j:Crash
    a owl:ObjectProperty ;
    rdfs:range j:CrashType ;
    rdfs:comment "A traffic accident." .

j:ChargeFelonyIndicator
    a owl:DataProperty ;
    rdfs:range xsd:boolean ;
    rdfs:comment "True if a charge refers to a felony offense; false otherwise." .

nc:ItemLengthMeasure
    a owl:ObjectProperty ;
    rdfs:range nc:LengthMeasureType ;
    rdfs:comment "A measurement of the length of an item." .

nc:Person
    a owl:ObjectProperty ;
    rdfs:range nc:PersonType ;
    rdfs:comment "A human being." .

nc:LatitudeDegreeValue
    a owl:DataProperty ;
    rdfs:range nc:LatitudeDegreeType ;
    rdfs:comment "A value that specifies the degree of a latitude. The value comes from a restricted range between -90 (inclusive) and +90 (inclusive)." .

hs:PersonOtherKinAssociationCategoryCode
    a owl:DataProperty ;
    rdfs:range hs:PersonOtherKinAssociationCodeType ;
    rdfs:comment "A code list that describes the nature of the kinship or other close personal relationship from a source person to a target person." .

nc:PersonName
    a owl:ObjectProperty ;
    rdfs:range nc:PersonNameType ;
    rdfs:comment "A combination of names and/or titles by which a person is known." .

nc:ReportedDate
    a owl:ObjectProperty ;
    rdfs:range nc:DateType ;
    rdfs:comment "A date information was observed, measured, identified, or became known." .

nc:Location2DGeospatialCoordinate
    a owl:ObjectProperty ;
    rdfs:subPropertyOf nc:LocationGeospatialCoordinateAbstract ;
    rdfs:range nc:Location2DGeospatialCoordinateType ;
    rdfs:comment "A location identified by a latitude and longitude." .

nc:MeasurePointAbstract
    a owl:DataProperty ;
    rdfs:comment "A data concept for a measurement value." .

j:CrashDriverType
    a owl:Class ;
    rdfs:subClass nc:PersonType ;
    rdfs:comment "A data type for a motor vehicle driver involved in a traffic accident." ;
    owl:subclassOf [
        a owl:Restriction ;
        owl:cardinality "1"^^xsd:nonNegativeInteger ;
        owl:onProperty j:DriverLicense
    ] .

nc:PersonNameType
    a owl:Class ;
    rdfs:comment "A data type for a combination of names and/or titles by which a person is known." .

hs:PersonOtherKinAssociationType
    a owl:Class ;
    rdfs:subClass nc:AssociationType ;
    rdfs:comment "A data type for a relationship that is a kinship or other close personal association between the source object and the target object. The relationship between a parent and a child should be captured using the ParentChildAssociation" .

j:DrivingIncidentType
    a owl:Class ;
    rdfs:subClass nc:IncidentType ;
    rdfs:comment "A data type for details of an incident involving a vehicle." .

priv:PrivacyMetadataType
    a owl:Class .

j:CrashVehicleType
    a owl:Class ;
    rdfs:comment "A data type for a motor vehicle involved in a traffic accident." ;
    owl:subclassOf [
        a owl:Restriction ;
        owl:cardinality "1"^^xsd:nonNegativeInteger ;
        owl:onProperty j:CrashDriver
    ] .

j:DriverLicenseBaseType
    a owl:Class ;
    rdfs:comment "A data type for an authorization issued to a driver granting driving privileges." .

exch:CrashDriverInfoType
    a owl:Class ;
    rdfs:comment "A data type for a collection of legal charges associated with the driver of a vehicle in a crash." ;
    owl:subclassOf [
        a owl:Restriction ;
        owl:cardinality "1"^^xsd:nonNegativeInteger ;
        owl:onProperty j:Crash
    ] .

nc:DateType
    a owl:Class ;
    rdfs:comment "A data type for a calendar date." ;
    owl:subclassOf [
        a owl:Restriction ;
        owl:cardinality "1"^^xsd:nonNegativeInteger ;
        owl:onProperty nc:DateRepresentation
    ] .

nc:MetadataType
    a owl:Class ;
    rdfs:comment "A data type for information that further qualifies primary data; data about data." .

nc:AssociationType
    a owl:Class ;
    rdfs:comment "A data type for an association, connection, relationship, or involvement somehow linking people, things, and/or activities together." .

j:DriverLicenseType
    a owl:Class ;
    rdfs:subClass j:DriverLicenseBaseType ;
    rdfs:comment "A data type for a license issued to a person granting driving privileges." ;
    owl:subclassOf [
        a owl:Restriction ;
        owl:cardinality "1"^^xsd:nonNegativeInteger ;
        owl:onProperty j:DriverLicenseCardIdentification
    ] .

nc:ActivityType
    a owl:Class ;
    rdfs:comment "A data type for a single or set of related actions, events, or process steps." .

j:CrashType
    a owl:Class ;
    rdfs:subClass j:DrivingIncidentType ;
    rdfs:comment "A data type for a traffic accident." ;
    owl:subclassOf [
        a owl:Restriction ;
        owl:minCardinality "1"^^xsd:nonNegativeInteger ;
        owl:onProperty j:CrashVehicle
    ] ;
    owl:subclassOf [
        a owl:Restriction ;
        owl:minCardinality "1"^^xsd:nonNegativeInteger ;
        owl:onProperty j:CrashPerson
    ] .

nc:LatitudeCoordinateType
    a owl:Class ;
    rdfs:comment "A data type for a measurement of the angular distance between a point on the Earth and the Equator." .

nc:LengthMeasureType
    a owl:Class ;
    rdfs:subClass nc:MeasureType ;
    rdfs:comment "A data type for a measure of a distance or extent." .

nc:MeasureType
    a owl:Class ;
    rdfs:comment "A data type for a measurement." .

hs:ParentChildAssociationType
    a owl:Class ;
    rdfs:subClass nc:AssociationType ;
    rdfs:comment "A data type for an association between a child and a person who is in a parent role toward that child." .

hs:ChildType
    a owl:Class ;
    rdfs:comment "A data type for information about a person who has not yet reached the age of legal majority (i.e., adulthood)." .

j:ChargeType
    a owl:Class ;
    rdfs:comment "A data type for a formal allegation that a specific person has committed a specific offense." .

nc:PersonType
    a owl:Class ;
    rdfs:comment "A data type for a human being." .

nc:LongitudeCoordinateType
    a owl:Class ;
    rdfs:comment "A data type for a measurement of the angular distance between a point on the Earth and the Prime Meridian." .

j:CrashPersonType
    a owl:Class ;
    rdfs:subClass nc:PersonType ;
    rdfs:comment "A data type for any person involved in a traffic accident." ;
    owl:subclassOf [
        a owl:Restriction ;
        owl:minCardinality "1"^^xsd:nonNegativeInteger ;
        owl:onProperty j:CrashPersonInjury
    ] .

j:PersonChargeAssociationType
    a owl:Class ;
    rdfs:subClass nc:AssociationType ;
    rdfs:comment "A data type for an association between a person and a charge." ;
    owl:subclassOf [
        a owl:Restriction ;
        owl:cardinality "1"^^xsd:nonNegativeInteger ;
        owl:onProperty nc:Person
    ] ;
    owl:subclassOf [
        a owl:Restriction ;
        owl:cardinality "1"^^xsd:nonNegativeInteger ;
        owl:onProperty j:Charge
    ] .

nc:IdentificationType
    a owl:Class ;
    rdfs:comment "A data type for a representation of an identity." .

nc:InjuryType
    a owl:Class ;
    rdfs:comment "A data type for a form of harm or damage sustained by a person." .

nc:Location2DGeospatialCoordinateType
    a owl:Class ;
    rdfs:comment "A data type for a location identified by latitude and longitude." ;
    owl:subclassOf [
        a owl:Restriction ;
        owl:cardinality "1"^^xsd:nonNegativeInteger ;
        owl:onProperty nc:GeographicCoordinateLatitude
    ] ;
    owl:subclassOf [
        a owl:Restriction ;
        owl:cardinality "1"^^xsd:nonNegativeInteger ;
        owl:onProperty nc:GeographicCoordinateLongitude
    ] .

nc:IncidentType
    a owl:Class ;
    rdfs:subClass nc:ActivityType ;
    rdfs:comment "A data type for an occurrence or an event that may require a response." .

nc:PersonAssociationType
    a owl:Class ;
    rdfs:subClass nc:AssociationType ;
    rdfs:comment "A data type for an association between people." .

nc:PersonUnionAssociationType
    a owl:Class ;
    rdfs:subClass nc:PersonAssociationType ;
    rdfs:comment "A data type for an association between two persons who are in a state of union with each other." .

nc:LocationType
    a owl:Class ;
    rdfs:comment "A data type for geospatial location." .
